more accurate name, originally given by max

new/make_array_naive.v
@@ -3,30 +3,30 @@ Require Import Arith Arith.Even Arith.Div2 List.
 Require Import Program.
 Require Import Omega.
 
-Inductive MakeArrayLinearR : list A -> bin_tree -> nat -> Prop :=
+Inductive MakeArrayNaiveR : list A -> bin_tree -> nat -> Prop :=
 | MALR_zero :
-    MakeArrayLinearR nil bt_mt 0
+    MakeArrayNaiveR nil bt_mt 0
 | MALR_succ :
     forall x xs bt bt' time insert_time,
       InsertR x bt bt' insert_time ->
-      MakeArrayLinearR        xs bt                  time ->
-      MakeArrayLinearR (x :: xs) bt' (time + insert_time).
-Hint Constructors MakeArrayLinearR.
+      MakeArrayNaiveR        xs bt                  time ->
+      MakeArrayNaiveR (x :: xs) bt' (time + insert_time).
+Hint Constructors MakeArrayNaiveR.
 
-Theorem MakeArrayLinearR_SequenceR :
+Theorem MakeArrayNaiveR_SequenceR :
   forall xs bt n,
-    MakeArrayLinearR xs bt n ->
+    MakeArrayNaiveR xs bt n ->
     SequenceR bt xs.
 Proof.
   intros xs bt n MALR.
   induction MALR; eauto.
   eapply InsertR_SequenceR; eauto.
 Qed.
-Hint Resolve MakeArrayLinearR_SequenceR.
+Hint Resolve MakeArrayNaiveR_SequenceR.
 
-Theorem make_array_linear :
+Theorem make_array_naive :
   forall xs,
-    { bt | exists n, MakeArrayLinearR xs bt n }.
+    { bt | exists n, MakeArrayNaiveR xs bt n }.
 Proof.
   induction xs as [| x xs]; [eauto |].
   destruct IHxs as [bt IR].
@@ -40,9 +40,9 @@ Proof.
   apply (MALR_succ _ _ bt); eauto.
 Defined.
 
-Theorem MakeArrayLinearR_Braun :
+Theorem MakeArrayNaiveR_Braun :
   forall xs bt n,
-    MakeArrayLinearR xs bt n ->
+    MakeArrayNaiveR xs bt n ->
     Braun bt (length xs).
 Proof.
   intro xs.
@@ -58,29 +58,29 @@ Proof.
   apply (IHxs bt0 time H0).
   assumption.
 Qed.
-Hint Resolve MakeArrayLinearR_Braun.
+Hint Resolve MakeArrayNaiveR_Braun.
 
-Theorem MakeArrayLinearR_correct :
+Theorem MakeArrayNaiveR_correct :
   forall xs bt n,
-    MakeArrayLinearR xs bt n ->
+    MakeArrayNaiveR xs bt n ->
     forall i x,
       IndexR bt i x ->
       ListIndexR xs i x.
 Proof.
   intros. eauto.
 Qed.
-Hint Resolve MakeArrayLinearR_correct.
+Hint Resolve MakeArrayNaiveR_correct.
 
-Theorem MakeArrayLinearR_time :
+Theorem MakeArrayNaiveR_time :
   forall xs bt t,
-    MakeArrayLinearR xs bt t ->
+    MakeArrayNaiveR xs bt t ->
     t = nlogn (length xs).
 Proof.
   intros xs bt t MALR.
   induction MALR; eauto.
   rename H into IR.
   subst.
-  apply MakeArrayLinearR_Braun in MALR.
+  apply MakeArrayNaiveR_Braun in MALR.
   eapply (InsertR_time _ _ _ _ _ MALR) in IR.
   subst.
   auto.
